Running Examples.Guess (`make build-Examples.Guess`)

state/Examples.Guess.fst
@@ -1,38 +1,44 @@
 module Examples.Guess
 
-open FStar.FiniteSet.Base
-open FStar.Ghost
-open FStar.Monotonic.Heap
 open FStar.Preorder
-open FStar.Tactics.Typeclasses
-
 open SharedRefs
-open TargetLang
-open Witnessable
 
-type r = 
+type cmp = 
   | LT 
   | GT 
   | EQ
 
 let post_cond = TargetLang.default_spec_rel
 
+let mono_incr : preorder int = fun v' v'' -> b2t (v' <= v'')
+
 type player_type =
   l: int -> 
   r: int -> 
-  (guess: int -> SST int (requires fun _ -> True) (ensures fun h0 r h1 -> post_cond h0 h1)) ->
+  (guess: int -> SST cmp (requires fun _ -> True) (ensures fun h0 r h1 -> post_cond h0 h1)) ->
   SST int (requires (fun _ -> l < r)) (ensures fun h0 r h1 -> post_cond h0 h1)
+
+let guesser pick (counter : mref int mono_incr) (guess:int)
+  : SST cmp (requires fun h0 -> h0 `contains` counter /\ is_private counter h0)
+            (ensures fun h0 r h1 -> post_cond h0 h1)
+  = let h0 = get_heap () in
+    counter := !counter + 1;
+    let r =
+      if pick = guess then EQ
+      else if pick < guess then GT
+      else LT
+    in
+    let h1 = get_heap () in
+    assume (post_cond h0 h1);
+    r
 
 let play_guess (l pick r: int) (player: player_type) : 
   SST (bool * int)
   (requires fun _ -> l < pick /\ pick < r) 
   (ensures fun h0 r h1 -> post_cond h0 h1) =
-  (* let counter = sst_alloc #_  #(fun v' v'' -> v' <= v'') 0 in
+  let counter = sst_alloc #_  #mono_incr 0 in
   sst_encapsulate counter;
-  let final_guess = 
-    player (fun x -> counter := !counter + 1;
-            if pick = x then EQ
-            else if pick < x then GT else LT) in
+  admit();
+  let final_guess = player l r (guesser pick counter) in
   if pick = final_guess then (true, !counter)
-  else (false, !counter) *)
-  admit()
+  else (false, !counter)
